crates/logic/hol/src/syntax/kind/mod.rs
@@ -1,0 +1,7 @@
+//! Kind constructors.
+
+mod arr;
+mod star;
+
+pub use arr::KindArr;
+pub use star::KindStar;
