crates/logic/hol/src/syntax/tm/mod.rs
@@ -1,0 +1,25 @@
+//! Term constructors.
+
+mod abs;
+mod app;
+mod bool;
+mod bv;
+mod eps;
+mod eq;
+mod fv;
+mod lam;
+mod link;
+mod rep;
+mod ty_exists;
+
+pub use abs::TmAbs;
+pub use app::TmApp;
+pub use bool::TmBool;
+pub use bv::TmBv;
+pub use eps::TmEps;
+pub use eq::TmEq;
+pub use fv::TmFv;
+pub use lam::TmLam;
+pub use link::TmLink;
+pub use rep::TmRep;
+pub use ty_exists::TyExists;
